progress

theories/Limits/Pullback.v
@@ -178,33 +178,37 @@ Section EquivPullback.
 
 End EquivPullback.
 
+
 (** Pullbacks commute with sigmas *)
 Section PullbackSigma.
 
-  Context {X : Type}
-          (A : X -> Type) (B : X -> Type) (C : X -> Type)
-          (f : forall x, B x -> A x) (g : forall x, C x -> A x).
+  Context
+    {X Y Z : Type}
+    {A : X -> Type} {B : Y -> Type} {C : Z -> Type}
+    (f : Y -> X) (g : Z -> X)
+    (r : forall x, B x -> A (f x))
+    (s : forall x, C x -> A (g x)).
 
   Definition equiv_sigma_pullback
-    : { x : X & Pullback (f x) (g x) }
-        <~> Pullback (functor_sigma idmap f) (functor_sigma idmap g).
+    : {p : Pullback f g & Pullback (transport A p.2.2 o r p.1) (s p.2.1)}
+      <~> Pullback (functor_sigma f r) (functor_sigma g s).
   Proof.
+    refine (_ oE (equiv_sigma_assoc _ _)^-1).
     refine (equiv_sigma_assoc _ _ oE _).
-    apply (equiv_functor_sigma' equiv_idmap).
-    intro x; apply (equiv_functor_sigma' equiv_idmap).
-    intro b; refine (equiv_sigma_assoc _ _ oE _).
+    apply (equiv_functor_sigma' equiv_idmap); intro y.
+    refine (_ oE (equiv_sigma_assoc _ _)^-1).
     refine (equiv_functor_sigma' equiv_idmap _ oE _).
-    { intro x'.
-      refine (equiv_functor_sigma' equiv_idmap _).
-      intro c; apply equiv_path_sigma. }
-    refine (equiv_functor_sigma' equiv_idmap (fun x' => _) oE _).
-    1: cbn; serapply equiv_sigma_symm.
-    refine ((equiv_sigma_assoc (paths x)
-      (fun l => {b0 : C l.1 & transport A l.2 (f x b) = g l.1 b0}))^-1 oE _).
-    symmetry.
-    refine (_ oE equiv_contr_sigma _).
-    reflexivity.
-Defined.
+    1: intro; apply equiv_sigma_assoc.
+    refine (equiv_sigma_symm _ oE _).
+    refine (equiv_functor_sigma' equiv_idmap _); intro z.
+    refine (_ oE _).
+    { refine (equiv_functor_sigma' equiv_idmap _); intro b.
+      refine (equiv_functor_sigma' equiv_idmap _); intro c.
+      apply equiv_path_sigma. }
+    refine (equiv_functor_sigma' equiv_idmap _ oE _).
+    1: intro b; cbn; apply equiv_sigma_symm.
+    cbn; apply equiv_sigma_symm.
+  Defined.
 
 End PullbackSigma.
 
